## Systems of Linear Equations

### Ex 1. 

Solve the system of equations:

$$
\begin{aligned} 2x+3y&=5,\\ x-4y&=-2. \end{aligned}
$$

using the methods: Cramer's rule, Gaussian elimination, and inverse matrix.

### Ex 2. 

Solve the system of three equations with three unknowns:

$$
\begin{aligned} x+y+z&=6,\\ 2x-y+3z&=14,\\ -x+2y-z&=-2. \end{aligned}
$$

using the methods: Cramer's rule, Gaussian elimination, and inverse matrix.

### Ex 3. 

$\star$ Consider the parametric system dependent on $\lambda$:

$$
\begin{aligned} x+\lambda y&=1,\\ 2x+(1+\lambda)y&=3. \end{aligned}
$$

Determine the values of $\lambda$ for which the system has one solution, infinitely many solutions, or no solution.

### Ex 4. 

For the coefficient matrix

$$
A=\begin{pmatrix}1 & 1 & 1\\ 0 & 2 & -1\\ 2 & -1 & 3\end{pmatrix}
$$

and the right-hand side vector $b=(4,1,3)^{\top}$, solve $Ax=b$ and check the result by substitution.


### Ex 5. 

Solve the systems of equations:

a)

$$
\begin{cases}
x_1 + 4x_2 + 3x_3 = 1, \\
2x_1 + 5x_2 + 4x_3 = 4, \\
x_1 - 3x_2 - 2x_3 = 5;
\end{cases}
$$

b)

$$
\begin{cases}
x_1 - 2x_2 - 3x_3 = 2, \\
x_1 - 4x_2 - 13x_3 = 14, \\
-3x_1 + 5x_2 + 4x_3 = 0;
\end{cases}
$$

c)

$$
\begin{cases}
x_1 - 2x_2 - 3x_3 = 2, \\
x_1 - 4x_2 - 13x_3 = 14, \\
-3x_1 + 5x_2 + 4x_3 = 2;
\end{cases}
$$

d)

$$
\begin{cases}
-4x_1 + 3x_2 + 2x_3 = -2, \\
5x_1 - 4x_2 + x_3 = 3;
\end{cases}
$$

e)

$$
\begin{cases}
-4x_1 + 3x_2 = 2, \\
5x_1 - 4x_2 = 0, \\
2x_1 - x_2 = a;
\end{cases}
$$

f)

$$
\begin{cases}
4x_1 + 5x_3 = 6, \\
x_2 - 6x_3 = -2, \\
3x_1 + 4x_3 = 3;
\end{cases}
$$

g)

$$
\begin{cases}
3x_1 - x_2 - 2x_3 = 2, \\
2x_2 - x_3 = -1, \\
3x_1 - 5x_2 = 3;
\end{cases}
$$

h)

$$
\begin{cases}
-x_1 + 2x_2 + 3x_3 = 0, \\
x_1 - 4x_2 - 13x_3 = 0, \\
-3x_1 + 5x_2 + 4x_3 = 0;
\end{cases}
$$


i)

$$
\begin{cases}
x_1 + x_2 + x_3 = 0, \\
2x_1 + 4x_2 + 3x_3 = 0, \\
4x_2 + 4x_3 = 0;
\end{cases}
$$

j)

$$
\begin{cases}
x_1 + x_2 + x_3 = -2, \\
2x_1 + 4x_2 - 3x_3 = 3, \\
4x_2 + 2x_3 = 2;
\end{cases}
$$

k)

$$
\begin{cases}
4x_1 + 4x_3 = 8, \\
x_2 - 6x_3 = -3, \\
3x_1 + x_2 - 3x_3 = 3;
\end{cases}
$$

l)

$$
\begin{cases}
5x_1 - 3x_2 = -7, \\
-2x_1 + 9x_2 = 4, \\
2x_1 + 4x_2 = -2;
\end{cases}
$$